02_FORMAL/coq/domains/mobile_os/GraphicsEngine.v
@@ -13,15 +13,17 @@
 From Stdlib Require Import Arith.Arith.
 From Stdlib Require Import Bool.Bool.
 From Stdlib Require Import Lists.List.
+From Stdlib Require Import ZArith.
 Import ListNotations.
 
 (** ** Core Definitions *)
 
 (** Time in microseconds *)
 Definition Microseconds : Type := nat.
+Definition FRAME_BUDGET_120HZ_US : Microseconds := Z.to_nat 8333%Z.
 
 (** Frame budget for 120Hz = 1/120 second = 8333 microseconds *)
-Definition frame_budget_120hz : Microseconds := 8333.
+Definition frame_budget_120hz : Microseconds := FRAME_BUDGET_120HZ_US.
 
 Record Frame : Type := mkFrame {
   frame_id : nat;
@@ -409,7 +411,7 @@ Qed.
 Theorem gpu_timeout_handled :
   forall (rt : RenderThread),
     well_formed_render_thread rt ->
-    rt_frame_time_us rt <= 8333.
+    rt_frame_time_us rt <= FRAME_BUDGET_120HZ_US.
 Proof.
   intros rt Hwf.
   destruct Hwf as [_ [_ Htime]]. exact Htime.
